More work on bounds

theories/L6_PCPS/bounds.v
@@ -3,26 +3,26 @@ Require Import Coq.NArith.BinNat Coq.Relations.Relations Coq.MSets.MSets Coq.MSe
 
 Require Import L6.cps L6.eval L6.cps_util L6.identifiers L6.ctx
         L6.Ensembles_util L6.List_util L6.size_cps L6.tactics L6.set_util
-        L6.logical_relations.
+        L6.logical_relations L6.logical_relations_cc.
 
 Import ListNotations.
 
 
 Section Bounds. 
 
-  Context (K : nat) (* basically the number of inlined applications *)
-          (M : nat). (* The total overhead of all L6 transformations *)
-
+  Context (K : nat) (* in essence, the number of inlined applications *)
+          (M : nat) (* The total overhead of all L6 transformations, generally different for each program *)
+          (Kpos : K > 0) (Mpos : M > 0).
   (* TODO: maybe remove step-index k if not needed in bounds *)
 
-  Definition upper_boundG (k : nat) : relation (exp * env *  nat) := 
+  Definition upper_boundG : relation (exp * env *  nat) := 
     fun '(e1, rho1, c1) '(e2, rho2, c2) => c2 <= M * c1.
 
-  Definition lower_boundG (k : nat) : relation (exp * env *  nat) := 
+  Definition lower_boundG : relation (exp * env * nat) := 
     fun '(e1, rho1, c1) '(e2, rho2, c2) => c1 <= K * c2.
 
-  Definition boundG (k : nat) : relation (exp * env *  nat) :=
-    relation_conjunction (lower_boundG k) (upper_boundG k).
+  Definition boundG : relation (exp * env *  nat) :=
+    relation_conjunction lower_boundG upper_boundG.
  
   Definition upper_boundL (local : nat) : relation nat := 
     fun c1 c2 => c2 + local <= M * c1.
@@ -33,6 +33,20 @@ Section Bounds.
   Definition boundL (local : nat) : relation nat :=
     relation_conjunction (lower_boundL local) (upper_boundL local).
   
+  (* Divergence preservation *)
+  Lemma cc_approx_exp_divergence pr cenv ct l e1 rho1 e2 rho2 :  
+    (forall k, cc_approx_exp pr cenv ct k (boundL l) boundG (e1, rho1) (e2, rho2)) ->
+    diverge pr cenv rho1 e1 -> 
+    diverge pr cenv rho2 e2.
+  Proof.
+    intros Hexp H1 c2. assert (Hd := H1). specialize (H1 (K*(c2 + l))).
+    edestruct Hexp as [v2 [c2' [Hs2 [Hp Hval]]]]. reflexivity. eassumption.
+    destruct v2; try contradiction.
+    assert (Hleq : c2 <= c2').
+    { destruct Hp as [Hp1 Hp2]. unfold lower_boundL in Hp1.  
+      eapply Nat_as_DT.mul_le_mono_pos_l in Hp1; eauto. omega. }
+    
+
 End Bounds.
 
   
